aneris/examples/reliable_communication/examples/hello_world/hello_world_proof.v
@@ -58,16 +58,14 @@ Section proof_of_the_code.
           RCParams_srv_saddr ⤳ (∅, ∅) ∗
         free_ports (ip_of_address RCParams_srv_saddr)
                    {[port_of_address RCParams_srv_saddr]} ∗
-        ⌜RCParams_srv_saddr ∈ A⌝ ∗
-        fixed A ∗
         SrvInit }}}
        server #RCParams_srv_saddr @[ip_of_address RCParams_srv_saddr]
     {{{ skt, RET skt; True }}}.
   Proof.
-    iIntros (Φ) "(#Hsi & Hmh & Hfp & Hf & Hit) HΦ".
+    iIntros (Φ) "(#Hsi & Hmh & Hfp & Hit) HΦ".
     rewrite /server.
     wp_lam.
-    wp_apply (RCSpec_make_server_skt_spec with "[$Hmh $Hfp $Hf $Hsi $Hit][HΦ]").
+    wp_apply (RCSpec_make_server_skt_spec with "[$Hmh $Hfp $Hsi $Hit][HΦ]").
     iNext. iIntros (skt) "Hcl".
     wp_pures.
     wp_apply (RCSpec_server_listen_spec with "[$Hcl][HΦ]").
@@ -86,19 +84,18 @@ Section proof_of_the_code.
 
   Lemma wp_client clt_addr :
     {{{ RCParams_srv_saddr ⤇ reserved_server_socket_interp ∗
-        ⌜clt_addr ∉ A⌝ ∗
         clt_addr ⤳ (∅, ∅) ∗
         free_ports (ip_of_address clt_addr)
                    {[port_of_address clt_addr]} ∗
-        fixed A }}}
+        unfixed {[clt_addr]} }}}
        client #clt_addr #srv_sa @[ip_of_address clt_addr]
     {{{ skt, RET skt; True }}}.
   Proof.
-    iIntros (Φ) "(#Hsi & #Hca & Hmh & Hfp & Hf) HΦ".
+    iIntros (Φ) "(#Hsi & Hmh & Hfp & Hf) HΦ".
     rewrite /client.
     wp_lam.
     wp_pures.
-    wp_apply (RCSpec_make_client_skt_spec with "[$Hmh $Hfp $Hca $Hsi $Hf][HΦ]").
+    wp_apply (RCSpec_make_client_skt_spec with "[$Hmh $Hfp $Hsi $Hf][HΦ]").
     iNext. iIntros (skt) "Hcl".
     wp_pures.
     wp_apply (RCSpec_connect_spec with "[$Hcl][HΦ]").
@@ -124,9 +121,7 @@ From aneris.examples.reliable_communication.instantiation
 (** Concrete parameters (addresses, ips) *)
 Definition srv_sa := SocketAddressInet "0.0.0.0" 80.
 Definition clt_sa := SocketAddressInet "0.0.0.1" 80.
-Definition A : gset socket_address := {[ srv_sa ]}.
 Definition ips : gset string := {[ "0.0.0.0" ; "0.0.0.1"]}.
-Lemma inA : srv_sa ∈ A. Proof. set_solver. Qed.
 
 Definition main : expr :=
     Start "0.0.0.0" (server #srv_sa) ;;
@@ -145,7 +140,7 @@ Section proof_of_the_main.
   Lemma main_spec :
     ⊢ |={⊤}=>
          srv_sa ⤇ @reserved_server_socket_interp _ _ _ UP SnRes -∗
-         fixed A -∗
+         unfixed {[clt_sa]} -∗
          free_ip "0.0.0.0" -∗
          free_ip "0.0.0.1" -∗
          SocketAddressInet "0.0.0.0" 80 ⤳ (∅, ∅) -∗
@@ -157,20 +152,20 @@ Section proof_of_the_main.
     destruct HsAPIn, HsAPIs.
     iIntros "".
     iModIntro.
-    iIntros "#Hsrv #Hfixed Hfree1 Hfree2 Hsa1 Hsa2 HSrvInit".
+    iIntros "#Hsrv Hf Hfree1 Hfree2 Hsa1 Hsa2 HSrvInit".
     rewrite /main.
     wp_apply aneris_wp_start; first done.
     iFrame "Hfree1".
     iSplitR "Hsa1 HSrvInit"; last first.
     { iNext. iIntros "Hfps".
-      iApply (@wp_server _ _ _ _ _ A _ SnRes chn _ with "[-]"); last done.
+      iApply (@wp_server _ _ _ _ _ _ SnRes chn _ with "[-]"); last done.
       by iFrame "#∗". }
     iNext. wp_pures.
     wp_apply aneris_wp_start; first done.
     iFrame "Hfree2".
     iSplit; first done.
     iNext. iIntros "Hfps".
-    iApply (@wp_client _ _ _ _ _ A _ SnRes chn _ _ clt_sa with "[-]");
+    iApply (@wp_client _ _ _ _ _ _ SnRes chn _ _ clt_sa with "[-]");
       last done.
     by iFrame "#∗".
   Qed.
@@ -196,8 +191,6 @@ From aneris.examples.reliable_communication.resources
 From aneris.examples.reliable_communication.spec
      Require Import ras resources.
 
-Definition fixed_dom : gset socket_address := {[ srv_sa ]}.
-
 Definition dummy_model := model unit (fun x y => True) ().
 
 Lemma dummy_model_finitary : adequacy.aneris_model_rel_finitary dummy_model.
@@ -217,31 +210,14 @@ Proof.
 Qed.
 
 From aneris.aneris_lang.program_logic Require Import aneris_adequacy.
-Definition socket_interp
-           `{ag: !anerisG empty_model Σ}
-           `{!SpecChanG Σ}
-           `{server_ghost_names}
-            (HinA : srv_sa ∈ fixed_dom)
-            (N : namespace)
-            (SnRes : SessionResources UP) sa : socket_interp Σ :=
-  (match sa with
-   | SocketAddressInet "0.0.0.0" 80 =>  @reserved_server_socket_interp _ _ ag UP SnRes
- (* @server_interp _ _ ag _ _ UP *)
-
-   | _ => λ msg, ⌜True⌝
-   end)%I.
 
 Theorem adequacy : aneris_adequate main "system" init_state (λ _, True).
 Proof.
   set (Σ := #[anerisΣ dummy_model; SpecChanΣ]).
-  eapply (@adequacy Σ dummy_model _ _ ips fixed_dom {[srv_sa; clt_sa]} ∅ ∅ ∅);
-    try done; last first.
-  { set_solver. }
-  { intros i. rewrite /ips !elem_of_union !elem_of_singleton.
-    intros [|]; subst; simpl; set_solver. }
-  { rewrite /ips /= !dom_insert_L dom_empty_L right_id_L //. }
-  iIntros (Hdg) "".
+  eapply (@adequacy Σ dummy_model _ _ ips {[clt_sa; srv_sa]} ∅ ∅ ∅);
+    try set_solver; last first.
   2:{ apply dummy_model_finitary . }
+  iIntros (Hdg) "".
   iMod (Reliable_communication_init_instance ⊤ UP)
     as (chn sgn SnRes) "(HsrvInit & Hspecs)"; [ solve_ndisj|].
   iDestruct "Hspecs"
@@ -251,15 +227,16 @@ Proof.
          & %Hlisten & %Haccept
          & %Hsend & %HsendTele
          & %HtryRecv & %Hrecv)".
-  iExists (socket_interp inA (nroot .@ "hw") SnRes).
   iMod (main_spec) as "Hmain".
   split; try done.
   split; try done.
   iModIntro.
-  iIntros "Hf Hsi Hb Hfg Hips _ _ _ _ _".
+  iIntros "Hf Hb Hfg Hips _ _ _ _ _".
   simpl in *.
-  iDestruct (big_sepS_delete _ _ srv_sa with "Hsi") as "[Hsi _]";
-    first set_solver.
+  iDestruct (unfixed_split with "Hf") as "[Hf Hf_srv]"; [set_solver|].
+  iApply (aneris_wp_socket_interp_alloc_singleton
+            (@reserved_server_socket_interp _ _ _ UP SnRes) with "Hf_srv").
+  iIntros "Hsi".
   iDestruct (big_sepS_delete _ _ "0.0.0.0" with "Hips") as "[Hip0 Hips]";
     first set_solver.
   iDestruct (big_sepS_delete _ _ "0.0.0.1" with "Hips") as "[Hip1 _]";
