aneris/examples/reliable_communication/examples/messages_in_order_loop/messages_in_order_loop_proof.v
@@ -103,15 +103,12 @@ Section proof_of_the_code.
           RCParams_srv_saddr ⤳ (∅, ∅) ∗
         free_ports (ip_of_address RCParams_srv_saddr)
                    {[port_of_address RCParams_srv_saddr]} ∗
-        ⌜RCParams_srv_saddr ∈ A⌝ ∗
-        fixed A ∗
         SrvInit }}}
        server #RCParams_srv_saddr @[ip_of_address RCParams_srv_saddr]
     {{{ RET #(); True }}}.
   Proof.
-    iIntros (Φ) "(#Hsi & Hmh & Hfp & %HinA & Hf & Hit) HΦ". rewrite /server. wp_pures.
-    wp_smart_apply (RCSpec_make_server_skt_spec with "[$Hmh $Hfp $Hf $Hsi $Hit][HΦ]"); first done.
-    iNext. iIntros (skt) "Hcl". wp_pures.
+    iIntros (Φ) "(#Hsi & Hmh & Hfp & Hit) HΦ". rewrite /server. wp_pures.
+    wp_smart_apply (RCSpec_make_server_skt_spec with "[$Hmh $Hfp $Hsi $Hit][HΦ]").    iNext. iIntros (skt) "Hcl". wp_pures.
     wp_apply (RCSpec_server_listen_spec with "[$Hcl][HΦ]").
     iNext. iIntros "Hp". wp_pures.
     wp_apply (aneris_wp_fork with "[-]").
@@ -121,15 +118,14 @@ Section proof_of_the_code.
 
   Lemma wp_client clt_addr (s1 s2 : string) :
     {{{ RCParams_srv_saddr ⤇ reserved_server_socket_interp ∗
-        ⌜clt_addr ∉ A⌝ ∗
         clt_addr ⤳ (∅, ∅) ∗
         free_ports (ip_of_address clt_addr) {[port_of_address clt_addr]} ∗
-        fixed A }}}
+        unfixed {[clt_addr]} }}}
        client #clt_addr #srv_sa #s1 #s2 @[ip_of_address clt_addr]
     {{{ skt, RET skt; True }}}.
   Proof.
-    iIntros (Φ) "(#Hsi & #Hca & Hmh & Hfp & Hf) HΦ". rewrite /client. wp_pures.
-    wp_apply (RCSpec_make_client_skt_spec with "[$Hmh $Hfp $Hca $Hsi $Hf][HΦ]").
+    iIntros (Φ) "(#Hsi & Hmh & Hfp & Hf) HΦ". rewrite /client. wp_pures.
+    wp_apply (RCSpec_make_client_skt_spec with "[$Hmh $Hfp $Hsi $Hf][HΦ]").
     iNext. iIntros (skt) "Hcl". wp_pures.
     wp_apply (RCSpec_connect_spec with "[$Hcl][HΦ]").
     iNext. iIntros (c) "Hc". wp_pures.
@@ -146,14 +142,13 @@ Section proof_of_the_code.
 
   Lemma wp_client_carpe_diem clt_addr (s1 s2 : string) :
     {{{ RCParams_srv_saddr ⤇ reserved_server_socket_interp ∗
-        ⌜clt_addr ∉ A⌝ ∗
         clt_addr ⤳ (∅, ∅) ∗
         free_ports (ip_of_address clt_addr) {[port_of_address clt_addr]} ∗
-        fixed A }}}
+        unfixed {[clt_addr]} }}}
        client_0 #clt_addr #srv_sa @[ip_of_address clt_addr]
     {{{ skt, RET skt; True }}}.
   Proof.
-    iIntros (Φ) "(#Hsi & #Hca & Hmh & Hfp & Hf) HΦ".  rewrite /client_0.
+    iIntros (Φ) "(#Hsi & Hmh & Hfp & Hf) HΦ".  rewrite /client_0.
     do 3 wp_pure _. by iApply (wp_client with "[$]").
     Qed.
 
@@ -193,7 +188,7 @@ Section proof_of_the_main.
   Lemma main_spec :
     ⊢ |={⊤}=>
          srv_sa ⤇ @reserved_server_socket_interp _ _ _ UP SnRes -∗
-         fixed A -∗
+         unfixed {[clt_sa0; clt_sa1]} -∗
          free_ip "0.0.0.0" -∗
          free_ip "0.0.0.1" -∗
          free_ip "0.0.0.2" -∗
@@ -207,7 +202,7 @@ Section proof_of_the_main.
     destruct HsAPIn, HsAPIs.
     iIntros "".
     iModIntro.
-    iIntros "#Hsrv #Hfixed Hfree1 Hfree2 Hfree3 Hsa1 Hsa2 Hsa3 HSrvInit".
+    iIntros "#Hsrv Hf Hfree1 Hfree2 Hfree3 Hsa1 Hsa2 Hsa3 HSrvInit".
     rewrite /main.
     wp_apply aneris_wp_start; first done.
     iFrame "Hfree1".
@@ -218,15 +213,16 @@ Section proof_of_the_main.
     iNext. wp_pures.
     wp_apply aneris_wp_start; first done.
     iFrame "Hfree2".
-    iSplitL "Hfree3 Hsa3".
+    iDestruct (unfixed_split with "Hf") as "[Hf0 Hf1]"; [set_solver|].
+    iSplitL "Hfree3 Hsa3 Hf1".
     - iNext. wp_pures. wp_apply aneris_wp_start; first done.
       + iFrame. iSplit; first done.
         iNext. iIntros "Hfps".
-        iApply (@wp_client _ _ _ _ _ _ SnRes chn _ _ A clt_sa1 with "[-]"); last done.
-        iFrame "#∗". iPureIntro. set_solver.
+        iApply (@wp_client _ _ _ _ _ _ SnRes chn _ _ clt_sa1 with "[-]"); last done.
+        iFrame "#∗".
     - iNext. iIntros "Hfi1".
-      iApply (@wp_client _ _ _ _ _ _ SnRes chn _ _ A clt_sa0 with "[-]"); last done.
-      iFrame "#∗". iPureIntro; set_solver.
+      iApply (@wp_client _ _ _ _ _ _ SnRes chn _ _ clt_sa0 with "[-]"); last done.
+      iFrame "#∗".
   Qed.
 
 End proof_of_the_main.
@@ -250,8 +246,6 @@ From aneris.examples.reliable_communication.resources
 From aneris.examples.reliable_communication.spec
      Require Import ras resources.
 
-Definition fixed_dom : gset socket_address := {[ srv_sa ]}.
-
 Definition dummy_model := model unit (fun x y => True) ().
 
 Lemma dummy_model_finitary : adequacy.aneris_model_rel_finitary dummy_model.
@@ -271,24 +265,11 @@ Proof.
 Qed.
 
 From aneris.aneris_lang.program_logic Require Import aneris_adequacy.
-Definition socket_interp
-           `{ag: !anerisG empty_model Σ}
-           `{!SpecChanG Σ}
-           `{server_ghost_names}
-            (HinA : srv_sa ∈ fixed_dom)
-            (N : namespace)
-            (SnRes : SessionResources UP) sa : socket_interp Σ :=
-  (match sa with
-   | SocketAddressInet "0.0.0.0" 80 =>  @reserved_server_socket_interp _ _ ag UP SnRes
- (* @server_interp _ _ ag _ _ UP *)
-
-   | _ => λ msg, ⌜True⌝
-   end)%I.
 
 Theorem adequacy : aneris_adequate main "system" init_state (λ _, True).
 Proof.
   set (Σ := #[anerisΣ dummy_model; SpecChanΣ]).
-  eapply (@adequacy Σ dummy_model _ _ ips fixed_dom {[srv_sa; clt_sa0; clt_sa1]} ∅ ∅ ∅);
+  eapply (@adequacy Σ dummy_model _ _ ips {[clt_sa0; clt_sa1; srv_sa]} ∅ ∅ ∅);
     try done; last first.
   { set_solver. }
   { intros i. rewrite /ips !elem_of_union !elem_of_singleton.
@@ -305,15 +286,16 @@ Proof.
          & %Hlisten & %Haccept
          & %Hsend & %HsendTele
          & %HtryRecv & %Hrecv)".
-  iExists (socket_interp inA (nroot .@ "hw") SnRes).
   iMod (main_spec) as "Hmain".
   split; try done.
   split; try done.
   iModIntro.
-  iIntros "Hf Hsi Hb Hfg Hips _ _ _ _ _".
+  iIntros "Hf Hb Hfg Hips _ _ _ _ _".
   simpl in *.
-  iDestruct (big_sepS_delete _ _ srv_sa with "Hsi") as "[Hsi _]";
-    first set_solver.
+  iDestruct (unfixed_split with "Hf") as "[Hf Hf_srv]"; [set_solver|].
+  iApply (aneris_wp_socket_interp_alloc_singleton
+            (@reserved_server_socket_interp _ _ _ UP SnRes) with "Hf_srv").
+  iIntros "Hsi".
   iDestruct (big_sepS_delete _ _ "0.0.0.0" with "Hips") as "[Hip0 Hips]";
     first set_solver.
   iDestruct (big_sepS_delete _ _ "0.0.0.1" with "Hips") as "[Hip1 Hips]";
